Test/civl/parallel1.bpl
@@ -24,10 +24,7 @@ procedure {:yields} {:layer 0} {:refines "AtomicSet"} Set(v: int);
 procedure {:yields} {:layer 1} PC()
 ensures {:layer 1} g == 3;
 {
-  yield;
   call Set(3);
-  yield;
-  assert {:layer 1} g == 3;
 }
 
 procedure {:yields} {:layer 1} PD()
