Test/civl/signature-mismatch.bpl
@@ -34,3 +34,9 @@ modifies x;
 { x := x'; }
 
 procedure {:yields} {:layer 0} {:refines "atomic_write_x_3"} write_x_3 ({:linear_in "lin"} x':int);
+
+function {:builtin "MapConst"} MapConstBool(bool) : [int]bool;
+function {:inline} {:linear "lin"} TidCollector(x: int) : [int]bool
+{
+  MapConstBool(false)[x := true]
+}
